verify simplified map kernel

pmap.v
@@ -5,9 +5,10 @@ Section Map.
 Local Notation TID := (Var 0).
 Local Notation BID := (Var 1).
 Local Notation ARR := (Var 2).
-Local Notation X := (Var 3).
-Local Notation Y := (Var 4).
-Local Notation I := (Var 5).
+Local Notation OUT := (Var 3).
+Local Notation X := (Var 4).
+Local Notation Y := (Var 5).
+Local Notation I := (Var 6).
 
 Variable ntrd : nat.
 Variable nblk : nat.
@@ -20,19 +21,22 @@ Local Close Scope exp_scope.
 
 Local Notation nt_gr := (nblk * ntrd).
 
-Definition inv (i : nat) (arr : Z) :=
+Definition inv (i : nat) (arr out : Z) (fout : nat -> Z) :=
   Ex ix, 
     !(ARR === arr) **
+    !(OUT === out) **
     !(I === Enum' (ix * nt_gr + i)) **
     !(Apure (ix * nt_gr + i < len + nt_gr)%nat) **
-    nth i (distribute nt_gr (Gl ARR) (ix * nt_gr) (fun i => f i + 1)%Z (nt_step nt_gr) 0) emp **
-    nth i (distribute nt_gr (Gl ARR) (len - (ix * nt_gr)) (fun i => f i) (nt_step nt_gr) (ix * nt_gr)) emp.
+    nth i (distribute nt_gr (Gl arr) (ix * nt_gr) f (nt_step nt_gr) 0) emp **
+    nth i (distribute nt_gr (Gl arr) (len - (ix * nt_gr)) f (nt_step nt_gr) (ix * nt_gr)) emp **
+    nth i (distribute nt_gr (Gl out) (ix * nt_gr) (fun i => f i + 1)%Z (nt_step nt_gr) 0) emp **
+    nth i (distribute nt_gr (Gl out) (len - (ix * nt_gr)) (fun i => fout i) (nt_step nt_gr) (ix * nt_gr)) emp.
 
-Definition map_ker (i : nat) (arr : Z) :=
+Definition map_ker (i : nat) (arr out : Z) (fout : nat -> Z):=
   I ::= (TID +C BID *C Z.of_nat ntrd);;
-  WhileI  (inv i arr) (I < Z.of_nat len) (
+  WhileI  (inv i arr out fout) (I < Z.of_nat len) (
     X ::= [Gl ARR +o I] ;;
-    [Gl ARR +o I] ::= X + 1%Z ;;
+    [Gl OUT +o I] ::= X + 1%Z ;;
     I ::= I +C Z.of_nat ntrd *C Z.of_nat nblk
   )%exp.
 
@@ -83,13 +87,16 @@ Qed.
 Hint Resolve nt_gr_neq_0 id_lt_nt_gr nf_lt.
 
 
-Lemma map_correct : forall (tid : Fin.t ntrd) (bid : Fin.t nblk) (arr : Z), 
+Lemma map_correct : forall (tid : Fin.t ntrd) (bid : Fin.t nblk) (arr out : Z) (fout : nat -> Z), 
   CSL (fun n => default ntrd) tid
   (!(ARR === arr) ** 
+   !(OUT === out) ** 
    List.nth (nf tid + nf bid * ntrd) (distribute nt_gr (Gl arr) len f (nt_step nt_gr) 0) emp **
+   List.nth (nf tid + nf bid * ntrd) (distribute nt_gr (Gl out) len fout (nt_step nt_gr) 0) emp **
    !(BID === zf bid) ** !(TID === zf tid))
-  (map_ker (nf tid + nf bid * ntrd) arr)
-  (List.nth (nf tid + nf bid * ntrd) (distribute nt_gr (Gl arr) len (fun x => f x + 1)%Z (nt_step nt_gr) 0) emp).
+  (map_ker (nf tid + nf bid * ntrd) arr out fout)
+  ( List.nth (nf tid + nf bid * ntrd) (distribute nt_gr (Gl arr) len f (nt_step nt_gr) 0) emp **
+    List.nth (nf tid + nf bid * ntrd) (distribute nt_gr (Gl out) len (fun v=>f v+1)%Z (nt_step nt_gr) 0) emp).
 Proof.
   (* assert (Htid : nat_of_fin tid < ntrd) by (destruct (Fin.to_nat _); simpl in *; auto). *)
   unfold map_ker; introv.
@@ -104,7 +111,9 @@ Proof.
       change_in H.
       { unfold_pures.
         sep_rewrite_in skip_arr_unfold' H; [|try first [omega | eauto]..]. 
-      2: nia.
+        2: nia.
+        sep_rewrite_in (@skip_arr_unfold' (nf tid + nf bid * ntrd) (Gl out)) H; [|try first [omega | eauto]..].
+        2: nia.
       apply H. } 
       sep_combine_in H. ex_intro x H. simpl in H. exact H. } Unfocus.
     
@@ -115,12 +124,19 @@ Proof.
       { intros s h H.
         sep_split_in H.
         change_in H.
-        { assert ((Gl ARR +o (Zn x * (Zn nblk * Zn ntrd) + (zf tid + zf bid * Zn ntrd))%Z ===l
-                  Gl ARR +o I)%exp s (emp_ph loc)).
+        { assert ((Gl arr +o (Zn x * (Zn nblk * Zn ntrd) + (zf tid + zf bid * Zn ntrd))%Z ===l
+                  Gl arr +o I)%exp s (emp_ph loc)).
           { unfold_pures; unfold_conn; simpl; f_equal; nia. }
-          sep_rewrite_in (mps_eq1) H; [|exact H0]. exact H. }
-          sep_combine_in H; exact H. } Unfocus.
+          sep_rewrite_in (mps_eq1) H; [|exact H0]. 
+          assert ((Gl out +o (Zn x * (Zn nblk * Zn ntrd) + (zf tid + zf bid * Zn ntrd))%Z ===l
+                  Gl out +o I)%exp s (emp_ph loc)).
+          { unfold_pures; unfold_conn; simpl; f_equal; nia. }
+          sep_lift_in H 3.
+          sep_rewrite_in (mps_eq1) H; [|exact H1]. 
+          sep_combine_in H; exact H. }
+        exact H. } Unfocus.
       hoare_forward; try (apply inde_distribute; auto; repeat (constructor; prove_indeE)).
+      
       intros ? ? H; apply H. }
     
     eapply rule_seq.
@@ -133,20 +149,26 @@ Proof.
       subA_normalize_in H. simpl in H. ex_intro v H. exact H. }
     
     unfold inv; intros s h H. destruct H as (v & H); simpl in H.
-    sep_split_in H. unfold_pures; subst.
+    sep_normal_in H; sep_split_in H.
+    unfold_pures; subst.
     exists (S x); autorewrite with sep.
     sep_split; try now (unfold_conn; simpl; auto; nia).
     sep_rewrite_r skip_arr_fold'; try omega; eauto.
-    sep_normal; simpl; repeat sep_cancel.
-    autorewrite with sep. repeat sep_cancel.
-    cuts_rewrite (len - (nt_gr + x * nt_gr) = len - x * nt_gr - nt_gr); auto.
-    zify; omega. }
+    sep_rewrite_r (@skip_arr_fold' (nf tid + nf bid * ntrd) (Gl (s OUT))); try omega; eauto.
+    sep_normal; simpl.
+    simpl; repeat sep_cancel.
+    cuts_rewrite (len - (nt_gr + x * nt_gr) = len - x * nt_gr - nt_gr); [|nia]. 
+    repeat autorewrite with sep. repeat sep_cancel. }
 
   { unfold inv; intros s h H. apply ex_lift_l_in in H as [x H]. sep_split_in H. unfold_pures.
-    rewrite HP1 in n; rewrite <-Nat2Z.inj_lt in n.
+    rewrite HP2 in n; rewrite <-Nat2Z.inj_lt in n.
     assert (len - x * nt_gr <= nf tid + nf bid * ntrd) by (zify; omega).
     assert (nf tid + nf bid * ntrd < nt_gr) by auto.
     apply scC in H; sep_rewrite_in nth_dist_nil H; try omega; eauto.
+    2: instantiate (1 :=len - x * nt_gr); intros j Hj; unfold nt_step.
+    2: rewrite plus_comm, Nat.mod_add; auto; rewrite Nat.mod_small; auto; try (zify; omega).
+    sep_normal_in H.
+    sep_lift_in H 2; sep_rewrite_in nth_dist_nil H; try omega; eauto.
     2: instantiate (1 :=len - x * nt_gr); intros j Hj; unfold nt_step.
     2: rewrite plus_comm, Nat.mod_add; auto; rewrite Nat.mod_small; auto; try (zify; omega).
     rewrite minus_diag in H; simpl in H.
@@ -165,68 +187,84 @@ Proof.
       rewrite mps_eq1; [|exact H2].
       split; intros; sep_cancel; apply IHn; auto.
     Qed.
-    assert ((Gl arr ===l Gl ARR) s (emp_ph loc)) by (unfold_conn; simpl; congruence).
-    sep_rewrite distribute_eq; eauto.
+    (* assert ((Gl arr ===l Gl ARR) s (emp_ph loc)) by (unfold_conn; simpl; congruence). *)
+    (* sep_rewrite distribute_eq; eauto. *)
     assert (x * nt_gr <= len \/ len < x * nt_gr) as [|] by omega.
     - apply scC in H; sep_rewrite_in nth_dist_ext H; try omega; auto.
       2: instantiate (1 :=len - x * nt_gr); intros j Hj; simpl; unfold nt_step;
          rewrite plus_comm, Nat.mod_add; auto; rewrite Nat.mod_small; auto; try omega.
+      sep_normal_in H.
+      sep_lift_in H 2; sep_rewrite_in nth_dist_ext H; try omega; auto.
+      2: instantiate (1 :=len - x * nt_gr); intros j Hj; simpl; unfold nt_step;
+         rewrite plus_comm, Nat.mod_add; auto; rewrite Nat.mod_small; auto; try omega.
       cutrewrite (x * nt_gr + (len - x * nt_gr) = len) in H; [|omega].
-
-      destruct leb; sep_normal_in H; sep_cancel.
+      destruct leb; sep_normal_in H; sep_split; try now (unfold_conn; simpl; auto); sep_cancel.
     - (* apply scC in H; sep_rewrite nth_dist_ext; try omega; auto. *)
       (* cutrewrite (len - x * ntrd = 0) in H; [|omega]. *)
       cutrewrite (x * nt_gr = len + (x * nt_gr - len)) in H; [|omega].
+      assert (forall j, j < x * nt_gr - len -> nt_step nt_gr (0 + len + j) <> nf tid + nf bid * ntrd).
+      { unfold nt_step; simpl; intros j Hj Hc.
+        assert (len + j + nt_gr < (S x) * nt_gr) by (simpl; omega).
+        assert (x * nt_gr + j + (nf tid + nf bid * ntrd) < len + j + nt_gr) by omega.
+        let t := (eval simpl in (Nat.mod_add (len + j) 1 nt_gr)) in pose proof t.
+        rewrite mult_1_l in H5.
+        rewrite (Nat.div_mod (len + j + nt_gr) nt_gr), H5 in H3, H4; auto.
+        assert (x * nt_gr  < nt_gr * ((len + j + nt_gr) / nt_gr)) by omega.
+        assert (nt_gr * ((len + j + nt_gr) / nt_gr) < S x * nt_gr) by omega.
+        rewrite mult_comm in H6; apply Nat.mul_lt_mono_pos_l in H6; try omega.
+        rewrite mult_comm in H7; apply Nat.mul_lt_mono_pos_r in H7; omega. } 
       sep_rewrite_in_r nth_dist_ext H; try omega; eauto.
-      destruct leb; sep_normal_in H; sep_cancel.
-      unfold nt_step; simpl; intros j Hj Hc.
-      assert (len + j + nt_gr < (S x) * nt_gr) by (simpl; omega).
-      assert (x * nt_gr + j + (nf tid + nf bid * ntrd) < len + j + nt_gr) by omega.
-      let t := (eval simpl in (Nat.mod_add (len + j) 1 nt_gr)) in pose proof t.
-      rewrite mult_1_l in H6.
-      rewrite (Nat.div_mod (len + j + nt_gr) nt_gr), H6 in H4, H5; auto.
-      assert (x * nt_gr  < nt_gr * ((len + j + nt_gr) / nt_gr)) by omega.
-      assert (nt_gr * ((len + j + nt_gr) / nt_gr) < S x * nt_gr) by omega.
-      rewrite mult_comm in H7; apply Nat.mul_lt_mono_pos_l in H7; try omega.
-      rewrite mult_comm in H8; apply Nat.mul_lt_mono_pos_r in H8; omega. }
+      sep_rewrite_in_r nth_dist_ext H; try omega; eauto.
+      sep_split; auto.
+      destruct leb; sep_normal_in H; repeat sep_cancel. }
 
   {  intros s h H; unfold inv; exists 0; simpl.
-     sep_split_in H; unfold_pures; sep_split.
-     - unfold_conn; simpl; eauto.
+     sep_split_in H; unfold_pures; sep_split; auto.
      - unfold_conn; simpl; autorewrite with sep; congruence.
      - unfold_conn. assert (nf tid + nf bid * ntrd < nt_gr) by auto. omega.
-     - assert ((Gl ARR ===l Gl arr) s (emp_ph loc)) by (unfold_conn; simpl; congruence).
-       sep_rewrite distribute_eq; eauto.
-       rewrite <-minus_n_O, nth_nseq; destruct leb; sep_normal; sep_cancel. }
+     - (* assert ((Gl ARR ===l Gl arr) s (emp_ph loc)) by (unfold_conn; simpl; congruence). *)
+       (* sep_rewrite distribute_eq; eauto. *)
+       rewrite <-minus_n_O, nth_nseq; destruct leb; sep_normal; sep_cancel.
+       
+  }
 Qed.
 
 Require Import Bdiv.
 Local Notation init := MyVector.init.
-Definition bth_pre (b : Fin.t nblk) (arr : val) :=
+Definition bth_pre (b : Fin.t nblk) (arr out : val) (fout : nat -> Z) :=
   !(ARR === arr) **
+  !(OUT === out) **
   conj_xs (ls_init 0 ntrd (fun i =>
-    skip_arr (Gl arr) 0 len nt_gr f (i + nf b * ntrd))).
+    skip_arr (Gl arr) 0 len nt_gr f (i + nf b * ntrd))) **
+  conj_xs (ls_init 0 ntrd (fun i =>
+    skip_arr (Gl out) 0 len nt_gr fout (i + nf b * ntrd))).
 
-Definition tr_pres (b : Fin.t nblk) (arr : val) := init (fun i : Fin.t ntrd =>
+Definition tr_pres (b : Fin.t nblk) (arr out : val) fout := init (fun i : Fin.t ntrd =>
   !(ARR === arr) ** 
+  !(OUT === out) ** 
   skip_arr (Gl arr) 0 len nt_gr f (nf i + nf b * ntrd) **
+  skip_arr (Gl out) 0 len nt_gr fout (nf i + nf b * ntrd) **
   !(BID === zf b)).
 
-Definition bth_post (b : Fin.t nblk) (arr : val) := 
+Definition bth_post (b : Fin.t nblk) (arr out : val) := 
   conj_xs (ls_init 0 ntrd (fun i  =>
-    skip_arr (Gl arr) 0 len nt_gr (fun v => f v + 1)%Z (i + nf b * ntrd))).
+    skip_arr (Gl arr) 0 len nt_gr f%Z (i + nf b * ntrd))) **
+  conj_xs (ls_init 0 ntrd (fun i  =>
+    skip_arr (Gl out) 0 len nt_gr (fun v => f v + 1)%Z (i + nf b * ntrd))).
 
-Definition tr_posts (b : Fin.t nblk) (arr : val) := (init (fun i : Fin.t ntrd =>
-  skip_arr (Gl arr) 0 len nt_gr (fun v => f v + 1)%Z (nf i + nf b * ntrd))).
+Definition tr_posts (b : Fin.t nblk) (arr out : val) := (init (fun i : Fin.t ntrd =>
+  skip_arr (Gl arr) 0 len nt_gr f (nf i + nf b * ntrd) **
+  skip_arr (Gl out) 0 len nt_gr (fun v => f v + 1)%Z (nf i + nf b * ntrd))).
 
 Definition E : env := fun v =>
   if var_eq_dec v BID then Lo
   else if var_eq_dec v ARR then Lo
+  else if var_eq_dec v OUT then Lo
   else Hi.  
 
 (* delete arguments of map_ker *)
 Definition map' : cmd.
-  pose (map_ker 0 0%Z) as map'; unfold map_ker, WhileI in map'; exact map'.
+  pose (map_ker 0 0%Z 0%Z (fun _:nat => 0%Z)) as map'; unfold map_ker, WhileI in map'; exact map'.
 Defined.
 
 Definition bspec : (barrier_spec ntrd) := fun i => (default ntrd).
@@ -236,10 +274,11 @@ Proof.
   unfold precise; intros; tauto.
 Qed.
 
-Lemma map_correct_b (b : Fin.t nblk) (arr : val) : 
-  CSLp ntrd E (bth_pre b arr ** !(BID === zf b)) map' (bth_post b arr).
+Lemma map_correct_b (b : Fin.t nblk) (arr out : val) (fout : nat -> Z) : 
+  CSLp ntrd E (bth_pre b arr out fout ** !(BID === zf b)) map' (bth_post b arr out).
 Proof.
-  applys (>> rule_par bspec (tr_pres b arr) (tr_posts b arr)); try first [omega | nia | eauto].
+  applys (>> rule_par bspec (tr_pres b arr out fout) (tr_posts b arr out));
+  try first [omega | nia | eauto].
   - destruct ntrd; eexists; try omega; eauto.
   - unfold bspec; split; intros; unfold default; simpl; rewrite MyVector.init_spec;
     unfold CSL.low_assn, low_assn, indeP; tauto.
@@ -247,49 +286,25 @@ Proof.
     apply precise_false.
   - unfold bth_pre, tr_pres; intros.
     sep_split_in H.
-    (* simplify the conclusion *)
-    apply sc_v2l.
-    rewrite (vec_to_list_init0 _ emp).
-    erewrite ls_init_eq0.
-    Focus 2.
-    { intros i Hi.
-      destruct (Fin.of_nat i ntrd) as [|Hex] eqn:Heq; [|destruct Hex; omega].
-      rewrite (Fin_nat_inv Heq). reflexivity. } Unfocus.
-    repeat sep_rewrite (@ls_star ntrd).
-    repeat sep_rewrite (@ls_pure ntrd); sep_split.
-    (* crush conditions for variables *)
-    apply ls_emp'; rewrite init_length; intros; rewrite ls_init_spec.
-    unfold TrueP; destruct lt_dec; eauto.
-    apply ls_emp'; rewrite init_length; intros; rewrite ls_init_spec.
-    unfold TrueP; destruct lt_dec; eauto.
-    
-    (* simplify the hypothesis *)
-    apply H.
-    (* rewrite (vec_to_list_init0 _ emp) in H. *)
-    (* erewrite ls_init_eq0 in H. *)
-    (* Focus 2. *)
-    (* { intros i Hi. *)
-    (*   destruct (Fin.of_nat i ntrd) as [|Hex] eqn:Heq; [|destruct Hex; omega]. *)
-    (*   rewrite (Fin_nat_inv Heq). reflexivity. } Unfocus. *)
-    (* eauto. *)
+    istar_simplify.
+    repeat sep_rewrite (@ls_star).
+    repeat sep_rewrite (@ls_pure).
+    sep_split.
+    apply ls_emp'; intros; rewrite ls_init_spec; destruct lt_dec; auto; cbv; auto.
+    apply ls_emp'; intros; rewrite ls_init_spec; destruct lt_dec; auto; cbv; auto.
+    apply ls_emp'; intros; rewrite ls_init_spec; destruct lt_dec; auto; cbv; auto.
+    repeat sep_cancel.
   - unfold tr_posts, bth_post; intros s h H.
-    apply sc_v2l in H.
-    rewrite (vec_to_list_init0 _ emp) in H.
-    erewrite ls_init_eq0 in H.
-    Focus 2.
-    { intros i Hi.
-      destruct (Fin.of_nat i ntrd) as [|Hex] eqn:Heq; [|destruct Hex; omega].
-      rewrite (Fin_nat_inv Heq). reflexivity. } Unfocus.
-    apply H.
+    istar_simplify_in H.
+    sep_cancel.
   - intros; unfold tr_pres; rewrite MyVector.init_spec.
     unfold CSL.low_assn.
     Hint Constructors typing_exp.
-    repeat prove_low_assn; eauto.
-    apply low_assn_skip_arr.
+    repeat prove_low_assn; eauto;
+    apply low_assn_skip_arr;
     constructor; eauto.
   - intros; unfold CSL.low_assn, tr_posts; rewrite MyVector.init_spec.
-    apply low_assn_skip_arr.
-    constructor; eauto.
+    prove_low_assn; apply low_assn_skip_arr; constructor; eauto.
   - repeat econstructor.
   - unfold tr_pres, tr_posts; intros; rewrite !MyVector.init_spec.
     unfold bspec, skip_arr.
@@ -299,7 +314,7 @@ Proof.
     intros.
     apply H.
     intros; sep_normal_in H; sep_normal; sep_cancel.
-
+    repeat sep_cancel; eauto.
     (* hmm.. *)
     Grab Existential Variables.
     apply Lo.
@@ -310,61 +325,30 @@ Proof.
     apply Lo.
 Qed.
 
-Definition bl_pres (arr : val) : Vector.t assn nblk :=
-  init (fun b : Fin.t nblk => (bth_pre b arr)).
-Definition bl_posts (arr : val) : Vector.t assn nblk :=
-  init (fun b : Fin.t nblk => (bth_post b arr)).
+Definition bl_pres (arr out : val) fout : Vector.t assn nblk :=
+  init (fun b : Fin.t nblk => (bth_pre b arr out fout)).
+Definition bl_posts (arr out : val) : Vector.t assn nblk :=
+  init (fun b : Fin.t nblk => (bth_post b arr out)).
 
-Theorem map_correct_g (arr : val) :
+Theorem map_correct_g (arr out : val) fout :
   CSLg ntrd nblk ntrd_neq0 nblk_neq0
-    (!(ARR === arr) ** 
-     is_array (Gl arr) len f 0)
+    (!(ARR === arr) ** !(OUT === out) ** 
+     is_array (Gl arr) len f 0 **
+     is_array (Gl out) len fout 0)
     (Pr nil map')
-    (is_array (Gl arr) len (fun v => f v + 1)%Z 0).
+    (is_array (Gl arr) len f 0 **
+     is_array (Gl out) len (fun v => f v + 1)%Z 0).
 Proof.
-  applys (>> rule_grid E (bl_pres arr) (bl_posts arr)).
+  applys (>> rule_grid E (bl_pres arr out fout) (bl_posts arr out)).
   - intros s h H.
     unfold bl_pres, bth_pre.
-    sep_split_in H; eauto.
-    
-    (* simplifying the conclusion *)
-    apply sc_v2l.
-    rewrite (vec_to_list_init0 _ emp).
-    erewrite ls_init_eq0.
-    Focus 2.
-    { intros i Hi.
-      destruct (Fin.of_nat i nblk) as [|Hex] eqn:Heq; [|destruct Hex; omega].
-      rewrite (Fin_nat_inv Heq).
-      reflexivity. } Unfocus.
+    sep_split_in H.
+    istar_simplify.
     repeat sep_rewrite (@ls_star nblk).
     repeat sep_rewrite (@ls_pure nblk); sep_split.
-    { apply ls_emp'; rewrite init_length; intros; rewrite ls_init_spec.
-      destruct lt_dec; eauto.
-      tauto. }
-    (* applys (>> equiv_from_nth emp). *)
-    (* Focus 2. *)
-    (* { intros i Hi stk. *)
-    (*   instantiate (1 := (ls_init 0 nblk *)
-    (*     (fun i0 : nat => *)
-    (*        conj_xs *)
-    (*          (ls_init 0 ntrd *)
-    (*             (fun i1 => *)
-    (*                skip_arr (Gl arr) 0 len nt_gr f (i1 + i0 * ntrd)))))). *)
-    (*   rewrite !ls_init_spec; destruct lt_dec. *)
-    (*   rewrite sc_v2l. *)
-    (*   rewrite (vec_to_list_init0 _ emp). *)
-    (*   erewrite ls_init_eq0. *)
-    (*   Focus 2. *)
-    (*   { intros j Hj. *)
-    (*     destruct (Fin.of_nat j ntrd) as [|Hex] eqn:Heq; [|destruct Hex; omega]. *)
-    (*     simpl. *)
-    (*     rewrite (Fin_nat_inv Heq). *)
-    (*     reflexivity. } Unfocus. *)
-    (*   reflexivity. *)
-    (*   reflexivity. } Unfocus. *)
-    (* rewrite !init_length; eauto. *)
-
-    apply is_array_skip_arr; eauto.
+    apply ls_emp'; intros; rewrite ls_init_spec; destruct lt_dec; auto; cbv; auto.
+    apply ls_emp'; intros; rewrite ls_init_spec; destruct lt_dec; auto; cbv; auto.
+    repeat (sep_rewrite_r is_array_skip_arr); eauto.
   - unfold bl_pres, bl_posts; intros.
     rewrite !MyVector.init_spec.
     eapply CSLp_backward.
@@ -374,35 +358,29 @@ Proof.
     intros; simpl in *; sep_normal_in H; eauto.
   - unfold bl_posts, bth_post.
     intros s h H.
-    apply sc_v2l in H.
-    rewrite (vec_to_list_init0 _ emp) in H.
-    erewrite ls_init_eq0 in H.
-    Focus 2.
-    { intros i Hi.
-      destruct (Fin.of_nat i nblk) as [|Hex] eqn:Heq; [|destruct Hex; omega].
-      rewrite (Fin_nat_inv Heq).
-      reflexivity. } Unfocus.
-    apply is_array_skip_arr in H; eauto.
+    istar_simplify_in H.
+    repeat sep_rewrite is_array_skip_arr; eauto.
   - prove_inde.
   - intros; unfold bl_pres, bth_pre.
     rewrite MyVector.init_spec.
-    prove_inde.
-    apply inde_conj_xs; rewrite init_length; intros.
-    rewrite ls_init_spec; destruct lt_dec; prove_inde.
+    prove_inde;
+    apply inde_conj_xs; rewrite init_length; intros;
+    rewrite ls_init_spec; destruct lt_dec; prove_inde;
     apply inde_distribute; prove_indeE.
   - intros bid; unfold bl_pres, bth_pre; rewrite MyVector.init_spec.
     Hint Constructors typing_exp typing_lexp.
-    repeat prove_low_assn; eauto.
-    apply low_assn_conj_xs; rewrite init_length; intros.
-    rewrite ls_init_spec; destruct lt_dec.
-    apply low_assn_skip_arr; eauto.
+    repeat prove_low_assn; eauto;
+    apply low_assn_conj_xs; rewrite init_length; intros;
+    rewrite ls_init_spec; destruct lt_dec; try prove_low_assn;
+    apply low_assn_skip_arr; eauto;
     prove_low_assn.
   - intros.
     unfold bl_posts, bth_post.
     rewrite MyVector.init_spec.
-    apply has_no_vars_conj_xs.
-    rewrite init_length; intros; rewrite ls_init_spec.
-    repeat has_no_vars_assn.
+    has_no_vars_assn;
+    apply has_no_vars_conj_xs;
+    rewrite init_length; intros; rewrite ls_init_spec;
+    repeat has_no_vars_assn;
     apply has_no_vars_skip_arr; simpl; eauto.
   - simpl; tauto.
   - unfold E; eauto.
@@ -412,5 +390,4 @@ Proof.
   - simpl; eauto.
 Qed.
     
-End Map
-.
+End Map.
