fold.v
@@ -886,53 +886,6 @@ Lemma barrier_wf bid : Bdiv.Aistar_v (fst (binv bid 1)) |= Bdiv.Aistar_v (snd (b
 Proof.
   simpl; intros s h H.
 
-  Ltac default T :=
-    lazymatch T with
-      | nat => constr:(0)
-      | Z => constr:(0%Z)
-      | ?T1 -> ?T2 => let t := default T2 in constr:(fun _ : T1 => t)
-    end.
-
-  Ltac ex_elim H :=
-    lazymatch type of H with
-      | conj_xs (ls_init _ _ (fun _ : nat => Ex _ : ?T, _)) _ _ =>
-        let t := default T in
-        sep_rewrite_in (@ls_exists0 _ t) H
-    end.
-
-  Ltac istar_simplify_in H :=
-    apply sc_v2l in H; rewrite (vec_to_list_init0 _ emp) in H; erewrite ls_init_eq0 in H;
-    [|let i := fresh "i" in
-      let Hi := fresh in
-      let Hex := fresh in
-      let Heq := fresh in
-      intros i Hi;
-      lazymatch goal with
-        [|- match ?X with inleft _ => _ | inright _ => _ end = _] =>
-        destruct X as [|Hex] eqn:Heq; [|destruct Hex; omega]
-      end;
-      rewrite (Fin_nat_inv Heq); reflexivity];
-    match goal with _ => idtac end;
-    (repeat (let vs := fresh "vs" in
-            ex_elim H; destruct H as [vs H]; sep_split_in H));
-    (repeat sep_rewrite_in (@ls_star) H);
-    (repeat sep_rewrite_in (@ls_pure) H; sep_split_in H).
- 
-
-  Ltac istar_simplify :=
-    apply sc_v2l; rewrite (vec_to_list_init0 _ emp); erewrite ls_init_eq0;
-    [|let i := fresh "i" in
-      let Hi := fresh in
-      let Hex := fresh in
-      let Heq := fresh in
-      intros i Hi;
-      lazymatch goal with
-        [|- match ?X with inleft _ => _ | inright _ => _ end = _] =>
-        destruct X as [|Hex] eqn:Heq; [|destruct Hex; omega]
-      end;
-      rewrite (Fin_nat_inv Heq); reflexivity];
-    match goal with _ => idtac end.
-
   istar_simplify_in H.
   istar_simplify.
   sep_rewrite (@ls_exists0 _ 0); exists vs; sep_split; eauto.
@@ -989,10 +942,7 @@ Proof.
         simpl in H''; destruct Nat.eq_dec; try omega.
         destruct (lt_dec (i + n') (n' * 2)); try omega.
         apply H''. 
-  - Ltac rewrite_body lem tac :=
-      erewrite ls_init_eq0; [|intros ? ?; rewrite lem; try tac; reflexivity ].
-    Ltac rewrite_body_in lem tac H :=
-      erewrite ls_init_eq0 in H; [|intros ? ?; rewrite lem; try tac; reflexivity ].
+  - 
     simpl in Hst.
     rewrite_body Hst omega.
     rewrite_body_in Hst omega H.
